working on dist syst

project02/DistributedSystem.t.dfy
@@ -22,24 +22,70 @@ module DistributedSystem {
       && (forall i:nat | i < |hosts| :: hosts[i].id == i)
     }
   }
+
   datatype Variables = Variables(
     hosts: seq<Host.Variables>,
     network: Network.Variables
   )
   {
     ghost predicate WF(c: Constants) {
-      && true
+      && c.WF()
+      && |hosts| == |c.hosts|
+      && forall i:nat | i < |hosts| :: hosts[i].WF(c.hosts[i])
     }
   }
 
+  // Initialize Init for Host and Network
   ghost predicate Init(c: Constants, v: Variables)
   {
-    && true   // define me
+    && v.WF(c)
+    && Network.Init(c.network, v.network)
+    && forall i:nat | i < |v.hosts| :: Host.Init(c.hosts[i], v.hosts[i])
   }
 
+  // TODO: Figure out how to repesent "Host Actions" with events (Get, Put) --> Noop is sending key,value pair
+  ghost predicate HostAction(c: Constants, v: Variables, v': Variables, hostid: HostId)
+  {
+    true // fix me
+  }
+
+  // Handling Put to update the Host's Variables (key and value)
+  function PutVariableUpdate(c: Constants, v: Variables, v': Variables, evt: Event) : Variables
+  {
+    // From network, find the Put message (which has the key and value to update)
+    // TODO: can there be multiple Put message in network? Or can we assume there will be a put message at this point?
+    var msg :| msg in v.network.inFlightMessages && msg.Put?;
+    
+    // From our hosts, find host with that key
+    
+
+    // Update this host's key with new value with the Put evt
+    // HandlePut(c: Constants, v: Variables, v': Variables, msgOps: MessageOps) 
+
+    
+    v
+  }
+
+  // Handling a Noop event, which means hosts are sharing key and value with other host
+  function NoOpVariableUpdate(c: Constants, v: Variables, v': Variables, evt: Event) : Variables
+  {
+    v
+  }
+
+  function ApplyEvents(c: Constants, v: Variables, v': Variables, evt: Event): Variables
+  {
+    // TODO: FIX MEEE
+    match evt
+      case Get(key, val) => v
+      case Put(key, val) => PutVariableUpdate(c, v, v', evt)
+      case NoOp => NoOpVariableUpdate(c, v, v', evt)
+    
+  }
+  // TODO: ask Ivan?
+  // Represent next step --> step is now event tho....
   ghost predicate Next(c: Constants, v: Variables, v': Variables, event: Event)
   {
-    true
+    v' == ApplyEvents(c, v, v', event)
   }
 /*}*/
 }
